Refactor and improve comments regarding type classes

theories/SOL/SOL.v
@@ -6,9 +6,10 @@ Definition vec := Vector.t.
 
 (* ** Syntax *)
 
+(* Parameterized over function and predicate signature as well as logical operators *)
 Class funcs_signature := { syms : Type; ar_syms : syms -> nat }.
 Class preds_signature := { preds : Type; ar_preds : preds -> nat }.
-Class operators := {binop : Type ; quantop : Type}.
+Class operators := { binop : Type ; quantop : Type }.
 
 Coercion syms : funcs_signature >-> Sortclass.
 Coercion preds : preds_signature >-> Sortclass.
@@ -25,7 +26,7 @@ Section Syntax.
 
   Inductive term : Type :=
     | var_indi : nat -> term
-    | func : forall ar, function ar -> vec term ar -> term.
+    | func : forall {ar}, function ar -> vec term ar -> term.
 
   Set Elimination Schemes.
 
@@ -39,7 +40,7 @@ Section Syntax.
 
   Inductive form : Type :=
     | fal : form
-    | atom : forall ar, predicate ar -> vec term ar -> form
+    | atom : forall {ar}, predicate ar -> vec term ar -> form
     | bin : binop -> form -> form -> form
     | quant_indi : quantop -> form -> form
     | quant_func : quantop -> nat -> form -> form
@@ -48,35 +49,11 @@ Section Syntax.
 End Syntax.
 
 Arguments var_func {_} _ {_}, {_} _ _.
-Arguments func {_ _}.
 Arguments var_pred {_} _ {_}, {_} _ _.
-Arguments atom {_ _ _ _}.
 
 
-(* ** Type class for 'cons' operation on environments *)
 
-Class Scons X := scons : X.
-Local Notation "x .: sigma" := (scons x sigma) (at level 70, right associativity).
-
-#[global]
-Instance scons_normal X : Scons (X -> (nat -> X) -> nat -> X) :=
-  fun x subst n => match n with
-                    | 0 => x
-                    | S n => subst n
-                  end.
-
-#[global]
-Instance scons_ar ar p : Scons (p ar -> (nat -> forall ar, p ar) -> nat -> forall ar, p ar) := fun f fi =>
-  fun n => match n with
-          | 0 => fun ar' => match Nat.eq_dec ar ar' with
-                            | left e => match e in _ = ar' return p ar' with eq_refl => f end
-                            | right _ => fi n ar'
-                            end
-          | S n => fun ar' => if Nat.eq_dec ar ar' then fi n ar' else fi (S n) ar'
-  end.
-
-
-(* ** Instantiate logical symbols to full SOL *)
+(* ** Instantiate logical operators to full SOL *)
 
 Inductive full_logic_sym : Type :=
 | Conj : full_logic_sym
@@ -91,55 +68,49 @@ Inductive full_logic_quant : Type :=
 Instance full_operators : operators :=
   {| binop := full_logic_sym ; quantop := full_logic_quant |}.
 
-Module SOLNotations.
-
-  Notation "x .: sigma" := (scons x sigma) (at level 70, right associativity).
-
-  Notation "$ x" := (var_indi x) (at level 5, format "$ '/' x").
-  Notation "i$ x" := (var_indi x) (at level 5, format "i$ '/' x").
-  Notation "f$ x" := (func (var_func x)) (at level 5, format "f$ '/' x").
-  Notation "p$ x" := (atom (var_pred x)) (at level 5, format "p$ '/' x").
-
-  Notation "⊥" := fal.
-  Notation "A ∧ B" := (@bin _ _ full_operators Conj A B) (at level 41).
-  Notation "A ∨ B" := (@bin _ _ full_operators Disj A B) (at level 42).
-  Notation "A '~>' B" := (@bin _ _ full_operators Impl A B) (at level 43, right associativity).
-  Notation "A '<~>' B" := ((A ~> B) ∧ (B ~> A)) (at level 43).
-  Notation "¬ A" := (A ~> ⊥) (at level 40).
-
-  Notation "∀i Phi" := (@quant_indi _ _ full_operators All Phi) (at level 50).
-  Notation "∃i Phi" := (@quant_indi _ _ full_operators Ex Phi) (at level 50).
-  Notation "∀f ( ar ) Phi" := (@quant_func _ _ full_operators All ar Phi) (at level 50).
-  Notation "∃f ( ar ) Phi" := (@quant_func _ _ full_operators Ex ar Phi) (at level 50).
-  Notation "∀p ( ar ) Phi" := (@quant_pred _ _ full_operators All ar Phi) (at level 50).
-  Notation "∃p ( ar ) Phi" := (@quant_pred _ _ full_operators Ex ar Phi) (at level 50).
-
-End SOLNotations.
-
 
 
 (* ** Tarski Semantics *)
 
 Section Tarski.
 
-  Context {Σ_funcs : funcs_signature}.
-  Context {Σ_preds : preds_signature}.
-
+  (* Environments *)
   Definition env_indi domain := nat -> domain.
   Definition env_func domain := nat -> forall ar, vec domain ar -> domain.
   Definition env_pred domain := nat -> forall ar, vec domain ar -> Prop.
   Record env domain := new_env { get_indi : env_indi domain ; get_func : env_func domain ; get_pred : env_pred domain }.
   Notation "⟨ a , b , c ⟩" := (new_env _ a b c).
 
-  Arguments get_indi {_} _ _.
-  Arguments get_func {_} _ _.
-  Arguments get_pred {_} _ _.
+  Arguments get_indi {_}.
+  Arguments get_func {_}.
+  Arguments get_pred {_}.
 
-  #[global] Instance scons_env_func domain ar : Scons _ := scons_ar ar (fun ar => vec domain ar -> domain).
-  #[global] Instance scons_env_pred domain ar : Scons _ := scons_ar ar (fun ar => vec domain ar -> Prop).
+  (* Extension operation on environments:  We use a type class here to support the 
+     same notation `x .: ρ` for individual, function, and predicate environments. *)
+  Class Econs X Env := econs : X -> Env -> Env.
+  Local Notation "x .: rho" := (econs x rho) (at level 70, right associativity).
+
+  #[global] Instance econs_indi domain : Econs domain (nat -> domain) :=
+    fun x env n => match n with  0 => x | S n => env n end.
+
+  (* Extension for function and predicate environments needs to take arity into account. *)
+  Definition econs_ar ar p : Econs (p ar) (nat -> forall ar, p ar) :=
+    fun x env n => match n with
+            | 0 => fun ar' => match Nat.eq_dec ar ar' with
+                              | left e => match e in _ = ar' return p ar' with eq_refl => x end
+                              | right _ => env n ar'
+                              end
+            | S n => fun ar' => if Nat.eq_dec ar ar' then env n ar' else env (S n) ar'
+    end.
+  #[global] Instance econs_func domain ar : Econs _ _ := econs_ar ar (fun ar => vec domain ar -> domain).
+  #[global] Instance econs_pred domain ar : Econs _ _ := econs_ar ar (fun ar => vec domain ar -> Prop).
+
+  Context {Σ_funcs : funcs_signature}.
+  Context {Σ_preds : preds_signature}.
 
   Variable domain : Type.
 
+  (* Interpretation of function and predicate symbols *)
   Class interp := B_I {
       i_f : forall f : syms, vec domain (ar_syms f) -> domain ;
       i_P : forall P : preds, vec domain (ar_preds P) -> Prop ;
@@ -181,13 +152,48 @@ Section Tarski.
 
 End Tarski.
 
+
+(* Boundle domain and interpretation into a model record *)
 Record Model `{funcs_signature, preds_signature} := { 
   M_domain : Type ;
   M_interp : interp M_domain
 }.
 
-Coercion M_interp : Model >-> interp.
+(* Allow to use a model M as a synonym for its domain and allow Coq 
+   to find interpretations inside models automatically. This allows us
+   to simply write `sat M rho phi`. *)
+Coercion M_domain : Model >-> Sortclass.
 #[global] Instance M_I `{funcs_signature, preds_signature} M : interp (M_domain M) := M_interp M.
+
+
+
+(* ** Notations for SOL *)
+
+Module SOLNotations.
+
+  Notation "x .: rho" := (econs x rho) (at level 70, right associativity).
+
+  Notation "$ x" := (var_indi x) (at level 5, format "$ '/' x").
+  Notation "i$ x" := (var_indi x) (at level 5, format "i$ '/' x").
+  Notation "f$ x" := (func (var_func x)) (at level 5, format "f$ '/' x").
+  Notation "p$ x" := (atom (var_pred x)) (at level 5, format "p$ '/' x").
+
+  Notation "⊥" := fal.
+  Notation "A ∧ B" := (@bin _ _ full_operators Conj A B) (at level 41).
+  Notation "A ∨ B" := (@bin _ _ full_operators Disj A B) (at level 42).
+  Notation "A '~>' B" := (@bin _ _ full_operators Impl A B) (at level 43, right associativity).
+  Notation "A '<~>' B" := ((A ~> B) ∧ (B ~> A)) (at level 43).
+  Notation "¬ A" := (A ~> ⊥) (at level 40).
+
+  Notation "∀i Phi" := (@quant_indi _ _ full_operators All Phi) (at level 50).
+  Notation "∃i Phi" := (@quant_indi _ _ full_operators Ex Phi) (at level 50).
+  Notation "∀f ( ar ) Phi" := (@quant_func _ _ full_operators All ar Phi) (at level 50).
+  Notation "∃f ( ar ) Phi" := (@quant_func _ _ full_operators Ex ar Phi) (at level 50).
+  Notation "∀p ( ar ) Phi" := (@quant_pred _ _ full_operators All ar Phi) (at level 50).
+  Notation "∃p ( ar ) Phi" := (@quant_pred _ _ full_operators Ex ar Phi) (at level 50).
+
+End SOLNotations.
+
 
 
 (* ** Instantiate empty signature *)
@@ -198,7 +204,7 @@ Coercion M_interp : Model >-> interp.
 (* ** List of decision problems *)
 
 (* Validity of formulas *)
-Definition SOL_valid (phi : form) := forall M rho, @sat _ _ (M_domain M) (M_interp M) rho phi.
+Definition SOL_valid (phi : form) := forall (M : Model) rho, sat M rho phi.
 
 (* Satisfiability of formulas *)
-Definition SOL_satis (phi : form) := exists M rho, @sat _ _ (M_domain M) (M_interp M) rho phi.
+Definition SOL_satis (phi : form) := exists (M : Model) rho, sat M rho phi.
